Second draft of Red_black_tree.v
	modified:   src/lib/Red_black_tree.v

src/lib/Red_black_tree.v
@@ -4,6 +4,7 @@ Require Import Coq.Lists.List.
 Import ListNotations.
 
 Set Implicit Arguments.
+Set Warnings "-extraction-opaque-accessed".
 
 
 (* Invariant:
@@ -108,6 +109,27 @@ Module M1 (S0: SORTABLE).
 
   Inductive Color: Set := Red | Black.
 
+  Definition is_Red (c:Color): Prop :=
+    match c with
+    | Red => True
+    | Black => False
+    end.
+
+  Definition is_Black (c:Color): Prop :=
+    match c with
+    | Red => False
+    | Black => True
+    end.
+
+  Theorem red_equal_black {A:Type} (eq:Red=Black): A.
+  Proof
+    ex_falso (Equal.use eq is_Red I).
+
+  Theorem black_equal_red {A:Type} (eq:Black=Red): A.
+  Proof
+    red_equal_black (Equal.flip eq).
+
+
   Inductive tree: Type :=
   | Leaf: tree
   | Node: Color -> tree -> S.t -> tree -> tree.
@@ -125,22 +147,37 @@ Module M1 (S0: SORTABLE).
       left I
     end.
 
+  Definition is_Node_red (t:tree): Prop :=
+    match t with
+    | Leaf => False
+    | Node c _ _ _ => is_Red c
+    end.
+
+  Definition is_Node_black (t:tree): Prop :=
+    match t with
+    | Leaf => False
+    | Node c _ _ _ => is_Black c
+    end.
+
+
   Definition color (t:tree): Color :=
     match t with
     | Leaf => Black
     | Node c _ _ _ => c
     end.
 
-  Theorem invert_tree:
-    forall {A:Type} {c:Color} {x:S.t} {u v:tree},
-      Leaf = Node c u x v -> A.
-  Proof.
-    refine (
-        fun A c x u v eq =>
-          let p := Equal.rewrite_bwd is_Node eq I in
-          match p with end
-      ).
-  Qed.
+  Theorem node_equal_leaf
+          {A:Type} {c:Color} {x:S.t} {u v:tree}
+          (eq:Node c u x v = Leaf): A.
+  Proof
+    ex_falso (Equal.use eq is_Node I).
+
+  Theorem leaf_equal_node
+          {A:Type} {c:Color} {x:S.t} {u v:tree}
+          (eq:Leaf = Node c u x v): A.
+  Proof
+    node_equal_leaf (Equal.flip eq).
+
 
   Theorem leaf_ne_node:
     forall (c:Color) (x:S.t) (u v:tree),
@@ -159,6 +196,69 @@ Module M1 (S0: SORTABLE).
     split. reflexivity. split. reflexivity. split;reflexivity.
   Qed.
 
+  Theorem node_injective2:
+    forall (c1 c2:Color) (x1 x2:S.t) (t1 t2 u1 u2:tree),
+      Node c1 t1 x1 u1 = Node c2 t2 x2 u2 ->
+      c1 = c2 /\ x1 = x2 /\ t1 = t2 /\ u1 = u2.
+  Proof.
+    refine(
+        let elem d t :=
+            match t with
+            | Leaf => d
+            | Node c t x u => x
+            end in
+        let left d t :=
+            match t with
+            | Leaf => d
+            | Node c t x u => t
+            end in
+        let right d t :=
+            match t with
+            | Leaf => d
+            | Node c t x u => u
+            end in
+        fun c1 c2 x1 x2 t1 t2 u1 u2 eq =>
+          let eqc: x1 = x2 := Equal.inject eq (elem x1) in
+          And.make4
+            (Equal.inject eq color)
+            (Equal.inject eq (elem x1))
+            (Equal.inject eq (left t1))
+            (Equal.inject eq (right t2))
+      ).
+  Qed.
+
+
+  Theorem use_node_equal:
+    forall {A:Prop} (c1 c2:Color) (x1 x2:S.t) (t1 t2 u1 u2:tree),
+      Node c1 t1 x1 u1 = Node c2 t2 x2 u2 ->
+      (c1=c2 -> x1=x2 -> t1=t2 -> u1=u2->A)
+      -> A.
+  Proof.
+    refine(
+        fun A c1 c2 x1 x2 t1 t2 u1 u2 eq P =>
+          let elem t :=
+              match t with
+              | Leaf => x1
+              | Node c t x u => x
+              end in
+          let left t :=
+              match t with
+              | Leaf => t1
+              | Node c t x u => t
+              end in
+          let right t :=
+              match t with
+              | Leaf => t2
+              | Node c t x u => u
+              end in
+          P (Equal.inject eq color)
+            (Equal.inject eq elem)
+            (Equal.inject eq left)
+            (Equal.inject eq right)
+      ).
+  Qed.
+
+
   Inductive Domain: tree -> S.t -> Prop :=
   | dom_singleton:
       forall c x,
@@ -174,22 +274,22 @@ Module M1 (S0: SORTABLE).
         x = y  -> Domain (Node c t y u) x.
 
 
-  Inductive RB_inv: nat -> Color -> tree -> Prop :=
-  | rb_leaf: RB_inv 0 Black Leaf
+  Inductive Red_black: nat -> Color -> tree -> Prop :=
+  | rb_leaf: Red_black 0 Black Leaf
   | rb_red:
       forall n t1 x t2,
-        RB_inv n Black t1 ->
-        RB_inv n Black t2 ->
-        RB_inv n Red (Node Red t1 x t2)
+        Red_black n Black t1 ->
+        Red_black n Black t2 ->
+        Red_black n Red (Node Red t1 x t2)
   | rb_black:
       forall n c1 t1 x c2 t2,
-        RB_inv n c1 t1 ->
-        RB_inv n c2 t2 ->
-        RB_inv (S n) Black (Node Black t1 x t2).
+        Red_black n c1 t1 ->
+        Red_black n c2 t2 ->
+        Red_black (S n) Black (Node Black t1 x t2).
 
   Theorem rb_inv_leaf:
     forall (h:nat) (c:Color),
-      RB_inv h c Leaf ->
+      Red_black h c Leaf ->
       h = 0 /\ c = Black.
   Proof.
     refine(
@@ -202,8 +302,8 @@ Module M1 (S0: SORTABLE).
 
   Theorem rb_inv_color:
     forall (h:nat) (c:Color) (t:tree),
-      RB_inv h c t ->
-      RB_inv h (color t) t.
+      Red_black h c t ->
+      Red_black h (color t) t.
   Proof.
     intros h c t rb.
     inversion rb as [ | | n c1 t1 x c2 t2 ].
@@ -214,7 +314,7 @@ Module M1 (S0: SORTABLE).
 
   Theorem use_rb_leaf:
     forall (h:nat) (c:Color),
-      RB_inv h c Leaf ->
+      Red_black h c Leaf ->
       forall (P:nat->Color->Prop),
         P 0 Black ->
         P h c.
@@ -229,9 +329,9 @@ Module M1 (S0: SORTABLE).
 
   Theorem use_rb_red:
     forall (h:nat) (x:S.t) (t1 t2:tree),
-      RB_inv h Red (Node Red t1 x t2) ->
+      Red_black h Red (Node Red t1 x t2) ->
       forall P:nat->tree->S.t->tree->Prop,
-        (RB_inv h Black t1 -> RB_inv h Black t2 -> P h t1 x t2) ->
+        (Red_black h Black t1 -> Red_black h Black t2 -> P h t1 x t2) ->
         P h t1 x t2.
   Proof.
     refine (
@@ -244,11 +344,11 @@ Module M1 (S0: SORTABLE).
 
   Theorem use_rb_black:
     forall (h:nat) (x:S.t) (t1 t2:tree),
-      RB_inv h Black (Node Black t1 x t2) ->
+      Red_black h Black (Node Black t1 x t2) ->
       forall (P:nat->tree->S.t->tree->Prop),
         (
-         RB_inv (pred h) (color t1) t1 ->
-         RB_inv (pred h) (color t2) t2 ->
+         Red_black (pred h) (color t1) t1 ->
+         Red_black (pred h) (color t2) t2 ->
          P h t1 x t2) ->
         P h t1 x t2.
   Proof.
@@ -262,6 +362,84 @@ Module M1 (S0: SORTABLE).
     - apply rb_inv_color with (c:=d2);assumption.
   Qed.
 
+  Theorem use_rb_black2:
+    forall (h:nat) (c:Color) (x:S.t) (t1 t2:tree),
+      Red_black h c (Node Black t1 x t2) ->
+      forall (P:nat->Color->tree->S.t->tree->Prop),
+        (
+         Red_black (pred h) (color t1) t1 ->
+         Red_black (pred h) (color t2) t2 ->
+         P h Black t1 x t2) ->
+        P h c t1 x t2.
+  Proof.
+    refine (
+        fun h c x t1 t2 inv =>
+          _
+      ).
+    inversion inv as [| | n d1 u1 y d2 u2 rb1 rb2 ].
+    intros P impl. apply impl.
+    - apply rb_inv_color with (c:=d1);assumption.
+    - apply rb_inv_color with (c:=d2);assumption.
+  Qed.
+
+
+
+  Theorem height_unique0: (* see below 'height_unique' *)
+    forall {h1 h2:nat} {c1 c2:Color} {t1 t2:tree},
+      Red_black h1 c1 t1 ->
+      Red_black h2 c2 t2 ->
+      t1 = t2 ->
+      h1 = h2.
+  Proof
+    fix f h1 h2 c1 c2 t1 t2 rb1:=
+    match rb1 with
+    | rb_leaf =>
+      fun rb2 =>
+        match rb2 with
+        | rb_leaf =>
+          fun _ => eq_refl
+        | rb_red _ _ _  =>
+          fun eq => leaf_equal_node eq
+        | rb_black _ _ _ =>
+          fun eq => leaf_equal_node eq
+        end
+    | rb_red _ rbu1 _ =>
+      fun rb2 =>
+        match rb2 with
+        | rb_leaf => fun eq => node_equal_leaf eq
+        | rb_red _ rbu2 _ =>
+          fun eq =>
+            use_node_equal
+              eq
+              (fun _ _ equ1 _ =>
+                 f _ _ _ _ _ _ rbu1 rbu2 equ1)
+        | rb_black _ rbu2 _ =>
+          fun eq =>
+            use_node_equal
+              eq
+              (fun rbeq => red_equal_black rbeq)
+        end
+    | rb_black x1 rbu1 rbv1 =>
+      fun rb2 =>
+        match rb2 with
+        | rb_leaf =>  fun eq => node_equal_leaf eq
+        | rb_red _ _ _ =>
+          fun eq =>
+            use_node_equal
+              eq
+              (fun breq => black_equal_red breq)
+        | rb_black _ rbu2 _ =>
+          fun eq =>
+            use_node_equal
+              eq
+              (fun _ _ equ1 _ =>
+                 Equal.inject
+                   (f _ _ _ _ _ _ rbu1 rbu2 equ1)
+                   S
+              )
+        end
+    end.
+
 
   Fixpoint black_height (t:tree): nat :=
     match t with
@@ -272,7 +450,7 @@ Module M1 (S0: SORTABLE).
 
   Theorem black_height_correct:
     forall (h:nat) (c:Color) (t:tree),
-      RB_inv h c t -> h = black_height t.
+      Red_black h c t -> h = black_height t.
   Proof
     fix f h c t rb :=
       match rb with
@@ -281,29 +459,163 @@ Module M1 (S0: SORTABLE).
       | rb_black x rb1 rb2 => Equal.inject (f _ _ _ rb1) S
       end.
 
+  Theorem height_unique:
+    forall {h1 h2:nat} {c1 c2:Color} {t:tree},
+      Red_black h1 c1 t ->
+      Red_black h2 c2 t ->
+      h1 = h2.
+  Proof
+    fun h1 h2 c1 c2 t rb1 rb2 =>
+      Equal.join
+        (black_height_correct rb1)
+        (Equal.flip (black_height_correct rb2)).
+
+
+  Theorem color_correct {h:nat} {c:Color} {t:tree} (rb:Red_black h c t)
+    : c = color t.
+  Proof
+      match rb in Red_black h c t return c = color t with
+      | rb_leaf => eq_refl
+      | rb_red x rb1 rb2 => eq_refl
+      | rb_black x rb1 rb2 => eq_refl
+      end.
+
+  Theorem color_unique {h1 h2:nat} {c1 c2:Color} {t:tree}
+      (rb1:Red_black h1 c1 t) (rb2:Red_black h2 c2 t): c1 = c2.
+  Proof
+    Equal.join (color_correct rb1) (Equal.flip (color_correct rb2)).
+
+
+  Theorem generalize_height_color:
+    forall  (h:nat) (c:Color) (t:tree) (P:nat->Color->Prop),
+      Red_black h c t ->
+      P h c ->
+      forall h c,
+        Red_black h c t -> P h c.
+  Proof
+    fun h c t P rb p h1 c1 rb1 =>
+      Equal.use2
+        (height_unique rb rb1:h=h1)
+        (color_unique  rb rb1:c=c1)
+        P p.
+
+  Theorem generalize_height:
+    forall  (h:nat) (c:Color) (t:tree) (P:nat->Prop),
+      Red_black h c t ->
+      P h ->
+      forall h,
+        Red_black h c t -> P h.
+  Proof
+    fun h c t P rb p h1 rb1 =>
+      @generalize_height_color
+        h c t
+        (fun h c => P h)
+        rb p h1 c rb1.
+
   Definition Same_black (t1 t2:tree): Prop :=
     black_height t1 = black_height t2.
 
-  Definition Red_black (t:tree): Prop :=
-    exists h, RB_inv h (color t) t.
+  Definition is_Red_black (t:tree): Prop :=
+    exists h, Red_black h (color t) t.
 
-  Inductive RB_nearly_inv: nat -> tree -> Prop :=
+  Theorem use_node_red_black:
+    forall (A:Prop) (c:Color) (x:S.t) (u v:tree),
+      is_Red_black (Node c u x v) ->
+      (is_Red_black u -> is_Red_black v -> A) ->
+      A.
+  Proof
+    fun A c x u v =>
+      match c with
+      | Red =>
+        fun rb =>
+          Exist.use
+            rb
+            (fun h (red:Red_black h Red (Node Red u x v)) f =>
+               use_rb_red
+                 red
+                 (fun h u x v => A)
+                 (fun rb1 rb2 =>
+                    let eqc1 := color_correct rb1 in
+                    let eqc2 := color_correct rb2 in
+                    let p1 := Equal.use eqc1 (fun c => Red_black _ c _) rb1 in
+                    let p2 := Equal.use eqc2 (fun c => Red_black _ c _) rb2 in
+                    f (ex_intro _ h p1) (ex_intro _ h p2)
+                 )
+            )
+      | Black =>
+        fun rb =>
+          Exist.use
+            rb
+            (fun h (blck:Red_black h Black (Node Black u x v)) f =>
+               use_rb_black
+                 blck
+                 (fun h u x v => A)
+                 (fun rb1 rb2 =>
+                    let eqc1 := color_correct rb1 in
+                    let eqc2 := color_correct rb2 in
+                    let p1 := Equal.use eqc1 (fun c => Red_black _ c _) rb1 in
+                    let p2 := Equal.use eqc2 (fun c => Red_black _ c _) rb2 in
+                    f (ex_intro _ (pred h) p1) (ex_intro _ (pred h) p2)
+                 )
+            )
+
+      end.
+
+  Theorem left_son_red_black:
+    forall (c:Color) (x:S.t) (u v:tree),
+      is_Red_black (Node c u x v) ->
+      is_Red_black u.
+  Proof
+    fun c x u v rb =>
+    use_node_red_black rb (fun rb1 rb2 => rb1).
+
+  Theorem right_son_red_black:
+    forall (c:Color) (x:S.t) (u v:tree),
+      is_Red_black (Node c u x v) ->
+      is_Red_black v.
+  Proof
+    fun c x u v rb =>
+    use_node_red_black rb (fun rb1 rb2 => rb2).
+
+
+
+
+
+
+  Inductive RB_nearly0: nat -> tree -> Prop :=
     nearly:
       forall n c1 t1 x c2 t2 c3,
-        RB_inv n c1 t1 ->
-        RB_inv n c2 t2 ->
-        RB_nearly_inv n (Node c3 t1 x t2).
+        Red_black n c1 t1 ->
+        Red_black n c2 t2 ->
+        RB_nearly0 n (Node c3 t1 x t2).
 
-  Definition RB_nearly (t:tree): Prop :=
-    exists h, RB_nearly_inv h t.
+  Inductive RB_nearly: nat -> tree -> Prop :=
+    rb_nearly:
+      forall n c1 t1 x c2 t2,
+        Red_black n c1 t1 ->
+        Red_black n c2 t2 ->
+        RB_nearly n (Node Red t1 x t2).
+
+
 
   Theorem singleton_nearly:
-    forall (c:Color) (x:S.t), RB_nearly_inv 0 (Node c Leaf x Leaf).
+    forall (c:Color) (x:S.t), RB_nearly0 0 (Node c Leaf x Leaf).
   Proof
         fun c x =>
           let t := Node c Leaf x Leaf in
           nearly x c rb_leaf rb_leaf.
 
+  Theorem use_rb_nearly_leaf:
+    forall (h:nat),
+      RB_nearly0 h Leaf ->
+      h = 0.
+  Proof.
+    intros h rbn.
+    inversion rbn.
+  Qed.
+
+  Definition is_Nearly (t:tree): Prop :=
+    exists h, RB_nearly0 h t.
 
   Inductive Rotation: tree -> tree -> Prop :=
   | rot_left:
@@ -360,16 +672,44 @@ Module M1 (S0: SORTABLE).
     inversion b. intros A impl. apply impl. assumption.
   Qed.
 
-  Theorem use_node_bounded:
-    forall (c:Color) (lo x hi:S.t) (t1 t2:tree),
+  Theorem use_node_bounded0:
+    forall {A:Prop} (c:Color) (lo x hi:S.t) (t1 t2:tree),
       Bounded lo (Node c t1 x t2) hi ->
-      forall (A:Prop) (P:Bounded lo t1 x -> Bounded x t2 hi -> A),
-        A.
+      (Bounded lo t1 x -> Bounded x t2 hi -> A) -> A.
   Proof.
-    intros c lo x hi t1 t2 b.
+    intros A c lo x hi t1 t2 b.
     inversion b.
-    intros A impl. apply impl;assumption.
+    intros impl. apply impl;assumption.
   Qed.
+
+
+  Theorem use_node_bounded:
+    forall {A:Prop} (c:Color) (lo x hi:S.t) (t1 t2:tree),
+      Bounded lo (Node c t1 x t2) hi ->
+      (Bounded lo t1 x -> Bounded x t2 hi -> A) -> A.
+  Proof
+    fun A c lo x hi t1 t2 b =>
+      let lemma lo t hi:
+            Bounded lo t hi ->
+            forall c t1 x t2,
+              t = Node c t1 x t2 ->
+              (Bounded lo t1 x -> Bounded x t2 hi -> A) -> A :=
+          fun b =>
+            match b with
+            | @leaf_bounded lo hi le =>
+              fun c t1 x t2 eq => leaf_equal_node eq
+            | @node_bounded lo t1 x t2 hi c b1 b2 =>
+              fun c0 u1 y u2 eq =>
+                use_node_equal
+                  eq
+                  (fun ceq xeq t1eq t2eq f =>
+                     f (Equal.use2 xeq t1eq (fun x t => Bounded lo t x) b1)
+                       (Equal.use2 xeq t2eq (fun x t => Bounded x t hi) b2)
+                  )
+            end
+      in
+      lemma lo (Node c t1 x t2) hi b c t1 x t2 eq_refl.
+
 
 
   Theorem bounds_le:
@@ -471,17 +811,54 @@ Module M1 (S0: SORTABLE).
     end.
 
   Definition Sorted (t:tree): Prop :=
-    is_Node t -> exists lo hi, Bounded lo t hi.
+    exists lo hi, Bounded lo t hi.
+
+  Theorem use_node_sorted:
+    forall (A:Prop) (c:Color) (x:S.t) (u v:tree),
+      Sorted (Node c u x v) ->
+      (Sorted u -> Sorted v -> A) ->
+      A.
+  Proof
+    fun A c x u v s =>
+      Exist.use2
+        s
+        (fun lo hi b =>
+           use_node_bounded
+             b
+             (fun b1 b2 =>
+                fun f =>
+                  f (Exist.make2 b1)
+                    (Exist.make2 b2))).
+
+  Theorem left_son_sorted:
+    forall (c:Color) (x:S.t) (u v:tree),
+      Sorted (Node c u x v) ->
+      Sorted u.
+  Proof
+    fun c x u v s =>
+      use_node_sorted
+        s (fun s1 s2 => s1).
 
 
-  Definition RB_sorted (t:tree): Prop := Red_black t /\ Sorted t.
+  Theorem right_son_sorted:
+    forall (c:Color) (x:S.t) (u v:tree),
+      Sorted (Node c u x v) ->
+      Sorted v.
+  Proof
+    fun c x u v s =>
+      use_node_sorted
+        s (fun s1 s2 => s2).
 
-  Definition RB_nearly_sorted (t:tree): Prop := RB_nearly t /\ Sorted t.
+
+
+  Definition RB_sorted (t:tree): Prop := is_Red_black t /\ Sorted t.
+
+  Definition RB_nearly_sorted (t:tree): Prop := is_Nearly t /\ Sorted t.
 
   Theorem singleton_sorted:
     forall (c:Color) (x:S.t), Sorted (Node c Leaf x Leaf).
   Proof
-    fun c x node =>
+    fun c x =>
       let le_xx: x <= x := S.reflexive x in
       let leafb: Bounded x Leaf x := leaf_bounded le_xx in
       let t := Node c Leaf x Leaf in
@@ -502,7 +879,7 @@ Module M1 (S0: SORTABLE).
       Lower_bound t lo ->
       Sorted t.
   Proof
-    fun t lo lb nd =>
+    fun t lo lb =>
       Exist.use lb (fun hi bnd => Exist.make2 bnd).
 
   Theorem upper_bound_to_sorted:
@@ -510,7 +887,7 @@ Module M1 (S0: SORTABLE).
       Upper_bound t hi ->
       Sorted t.
   Proof
-    fun t hi hb nd =>
+    fun t hi hb =>
       Exist.use hb (fun ls bnd => Exist.make2 bnd).
 
 
@@ -570,7 +947,7 @@ Module M1 (S0: SORTABLE).
       Lower_bound t2 x ->
       Sorted (Node c t1 x t2).
   Proof
-    fun c t1 x t2 hb lb nd =>
+    fun c t1 x t2 hb lb =>
       let le_xx: x <= x := S.reflexive x in
       Exist.use
         hb
@@ -646,28 +1023,28 @@ Module M1 (S0: SORTABLE).
 
 
 
-  Inductive Insert: S.t -> tree -> tree -> Prop :=
+  Inductive Inserted: S.t -> tree -> tree -> Prop :=
   | ins_leaf:
-      forall c x, Insert x Leaf (Node c Leaf x Leaf)
+      forall c x, Inserted x Leaf (Node c Leaf x Leaf)
   | ins_left:
       forall c x y t1 t1new t2,
         x <= y ->
-        Insert x t1 t1new ->
-        Insert x (Node c t1 y t2) (Node c t1new y t2)
+        Inserted x t1 t1new ->
+        Inserted x (Node c t1 y t2) (Node c t1new y t2)
   | ins_right:
       forall c x y t1 t2 t2new,
         y <= x ->
-        Insert x t2 t2new ->
-        Insert x (Node c t1 y t2) (Node c t1 y t2new)
+        Inserted x t2 t2new ->
+        Inserted x (Node c t1 y t2) (Node c t1 y t2new)
   | ins_replace:
       forall c x y t1 t2,
         S.Equivalent x y ->
-        Insert x (Node c t1 y t2) (Node c t1 x t2)
+        Inserted x (Node c t1 y t2) (Node c t1 x t2)
   | ins_rotation:
       forall x t1 t2 t3,
-        Insert x t1 t2 ->
+        Inserted x t1 t2 ->
         Rotation t2 t3 ->
-        Insert x t1 t3.
+        Inserted x t1 t3.
 
 
 
@@ -683,7 +1060,7 @@ Module M1 (S0: SORTABLE).
 
   Theorem insert_to_bounded:
     forall (x:S.t) (t1 t2:tree),
-      Insert x t1 t2 ->
+      Inserted x t1 t2 ->
       forall lo hi,
         lo <= x ->
         x <= hi ->
@@ -740,15 +1117,15 @@ Module M1 (S0: SORTABLE).
 
 
 
-  Definition RBT: Type := {t:tree | Red_black t}.
+  Definition RBT: Type := {t:tree | is_Red_black t}.
 
-  Definition RBN: Type := {t:tree | exists h, RB_nearly_inv h t}.
+  Definition RBN: Type := {t:tree | exists h, RB_nearly0 h t}.
 
   Theorem nearly_leaf_to_absurd:
-    forall (h:nat), RB_nearly_inv h Leaf -> False.
+    forall (h:nat), RB_nearly0 h Leaf -> False.
   Proof.
     refine (
-      let f: forall h t, RB_nearly_inv h t -> t = Leaf -> False :=
+      let f: forall h t, RB_nearly0 h t -> t = Leaf -> False :=
           fun _ _ nrb =>
             match nrb with
               nearly _ _ _ _ =>
@@ -763,13 +1140,13 @@ Module M1 (S0: SORTABLE).
 
   Theorem nearly_node_to_rb:
     forall (h:nat) (c:Color) (t1:tree) (x:S.t) (t2:tree),
-      RB_nearly_inv h (Node c t1 x t2) ->
-      RB_inv (S h) Black (Node Black t1 x t2).
+      RB_nearly0 h (Node c t1 x t2) ->
+      Red_black (S h) Black (Node Black t1 x t2).
   Proof.
     refine (
         let f: forall h t c t1 x t2,
-            RB_nearly_inv h t -> t = Node c t1 x t2 ->
-            RB_inv (S h) Black (Node Black t1 x t2) :=
+            RB_nearly0 h t -> t = Node c t1 x t2 ->
+            Red_black (S h) Black (Node Black t1 x t2) :=
             fun h t c t1 x t2 nrb =>
               match nrb with
                 @nearly h2 ca ta z cb tb c3 rba rbb =>
@@ -791,7 +1168,7 @@ Module M1 (S0: SORTABLE).
           exist _ t rbn =>
           (match t with
            | Leaf =>
-             let f: forall t, (exists h,RB_nearly_inv h t) -> t = Leaf -> False :=
+             let f: forall t, (exists h,RB_nearly0 h t) -> t = Leaf -> False :=
                  fun t rbn =>
                    match rbn with
                      ex_intro _ h nrb =>
@@ -805,7 +1182,7 @@ Module M1 (S0: SORTABLE).
            | Node c t1 x t2 =>
              fun rbn =>
                let t := Node Black t1 x t2 in
-               let rbt: exists h, RB_inv h Black t :=
+               let rbt: exists h, Red_black h Black t :=
                    match rbn with
                      ex_intro _ h rb =>
                      let q := @nearly_node_to_rb h c t1 x t2 rb in
@@ -821,11 +1198,11 @@ Module M1 (S0: SORTABLE).
 
 
 
-  Definition make_black2 (t:tree): RB_nearly t -> RBT.
+  Definition make_black2 (t:tree): is_Nearly t -> RBT.
     refine (
         match t with
         | Leaf =>
-          let f: forall t, (exists h,RB_nearly_inv h t) -> t = Leaf -> False :=
+          let f: forall t, (exists h,RB_nearly0 h t) -> t = Leaf -> False :=
               fun t rbn =>
                 match rbn with
                   ex_intro _ h nrb =>
@@ -839,7 +1216,7 @@ Module M1 (S0: SORTABLE).
         | Node c t1 x t2 =>
           fun rbn =>
             let t := Node Black t1 x t2 in
-            let rbt: exists h, RB_inv h Black t :=
+            let rbt: exists h, Red_black h Black t :=
                 match rbn with
                   ex_intro _ h rb =>
                   let q := @nearly_node_to_rb h c t1 x t2 rb in
@@ -853,128 +1230,178 @@ Module M1 (S0: SORTABLE).
   Defined.
 
 
+  (*====================================*)
+  (** * Insertion *)
+  (*====================================*)
+
+
+
+  (* A third definition for insertions
+     ---------------------------------*)
+
 
   Definition Insert_result (x:S.t) (t:tree): Type :=
-    {u:tree | Red_black t -> Sorted t -> Red_black u /\ Insert x t u}.
+    {u:tree | is_Red_black u /\ Inserted x t u}. (* inserted implies sorted *)
+
+  Definition Ins_red_balanced (x:S.t) (t u:tree): Prop :=
+    forall h, Red_black h Red t -> RB_nearly0 h u.
+
+  Definition Ins_black_balanced (x:S.t) (t u:tree): Prop :=
+    forall h, Red_black h Black t -> Red_black h (color u) u.
+
+  Definition Ins_balanced (x:S.t) (t u:tree): Prop :=
+    Ins_red_balanced x t u \/ Ins_black_balanced x t u.
+
+  Definition Ins_result (x:S.t) (t u:tree): Prop :=
+    Inserted x t u /\
+    Ins_balanced x t u.
+
+
+  Definition Black_son_inserted
+             (x:S.t) (t u v w:tree)
+    : Prop :=
+    (* t is a black tree and one of the sons of v. x has been inserted into t
+    and the result is u. Therefore u is sorted and balanced. The proposition
+    states that x is inserted into v resulting in w where w is nearly
+    balanced.*)
+    forall c h lo hi,
+      lo <= x ->
+      x <= hi ->
+      Inserted x t u ->
+      Bounded lo u hi ->
+      Red_black h c u ->
+      Inserted x v w /\ RB_nearly0 h w.
+
+  Definition Red_son_inserted
+             (x:S.t) (t u v w:tree)
+    : Prop :=
+    (* t is a red tree and one of the sons of v. x has been inserted into t
+    resulting in u. Therefore u is sorted, red and nearly balanced (maybe
+    fully balanced). The proposition states that x has been inserted into v
+    resulting in w where w is balanced. The color of w can be red or black. If
+    u is balanced then the color can stay black as the color of v. If u has a
+    red son and grandson then the blackness of v might have been pushed down
+    and w might be red.*)
+    forall h lo hi,
+      lo <= x ->
+      x <= hi ->
+      Inserted x t u ->
+      Bounded lo u hi ->
+      is_Node_red u ->
+      RB_nearly0 h u ->
+      Inserted x v w /\ exists c, Red_black (S h) c w.
+
+
+
+  (** ins: forall t, is_Red_black t -> Sorted t -> Ins_result x t u
+
+  'ins' gets a sorted redblack tree and returns an inserted and possibly
+  rebalanced tree.
+
+  Insertion into a node (t1 y' t2) either into the left or right son. 'ins t0
+  rb0 s0' returns Ins_result x' ta ua where ta is either t1 or t2.
+
+  There are two cases needing rebalancing:
+
+  a) u0 = N R (N R a x b) y c
+
+  b) u0 = N R a x (N R b y c)
+
+  Since is_Nearly u0, Ins_result x ta ua must be the case Ins_red_balanced x'
+  ta ua, i.e. ta must be red and the original tree (t1 y' t2) must be
+  black. All subtrees a b c have height h where h is the height of ta. The
+  other son of the original tree tb must have the same height. The rebalanced
+  trees are
+
+      N R (N B a x b) y (N B c y' tb) -- tb is the right son
+
+      N R (N B tb y' a) x (N B b y c) -- tb is the left son
+
+  The original tree has height 1+h and the rebalanced as well. Therefore we
+  can return Ins_black_balanced x' t u which is a valid Ins_result.
+
+  All the other cases don't need rebalancing. We have to prove this case by case.
+
+
+  This case is impossible, because x' has been inserted into t0.
+
+  The remaining case are nodes. After the rebalance cases there remain:
+
+  a) u0 = Leaf                          -- impossible, no insertion
+  b) u0 = N B a x b                     -- original black, balanced
+  c) u0 = N R Leaf x Leaf               -- insertion into empty tree
+  d) u0 = N R Leaf x (N B b y c)        -- impossible: neither nearly nor balanced
+  e) u0 = N R (N B a x b) y Leaf        -- impossible: neither nearly nor balanced
+  f) u0 = N R (N B a x b) y (N B c z d) -- balanced
+
+   *)
+
+  Theorem rebalance:
+    forall (x0:S.t) (t0 u0:tree),
+      is_Red_black t0 ->
+      Sorted t0 ->
+      Inserted x0 t0 u0 ->
+      Ins_balanced x0 t0 u0 ->
+      False.
+  Proof
+    fun x0 t0 u0 =>
+      match u0 with
+      | Node Red (Node Red a x b) y c => _
+      | Node Red a x (Node Red b y c) => _
+      | Leaf => _
+      | Node Black a x b => _
+      | Node Red Leaf x Leaf => _
+      | Node Red Leaf x (Node Black b y c) => _
+      | Node Red (Node Black a x b) y Leaf => _
+      | Node Red (Node Black a x b) y (Node Black c z d) => _
+      end.
 
   Import Relation.
 
   Definition insert
-             (x:S.t) (t:tree): Insert_result x t :=
-    let Res0 t :=
-        {u |
-         forall lo hi h c,
-           Bounded lo t hi ->
-           RB_inv h c t ->
-           RB_nearly_inv h u /\ Insert x t u} in
-    let bal_left c t1 (r1:Res0 t1) z t2: Res0 (Node c t1 z t2) :=
-        Sigma.use
-          r1
-          (fun u1 p1 =>
-             match c return Res0 (Node c t1 z t2) with
-             | Red => _
-             | Black =>
-               match u1 with
-               | Node Red (Node Red a x b) y c => _
-               | Node Red a x (Node Red b y c) => _
-               | _ => _
-               end
-             end
-          )
-    in
-    let bal_right c t1 y t2  (r2:Res0 t2): Res0 (Node c t1 y t2) :=
-        _
-    in
-    let sub c t1 y t2 (xy:x<=y) (yx:y<=x): Res0 (Node c t1 y t2) :=
-        _
-    in
-    let ins: forall t,  Res0 t :=
+             (x:S.t) (t:tree)
+    : is_Red_black t -> Sorted t -> Insert_result x t :=
+    let ins: forall t,
+        is_Red_black t -> Sorted t ->  {u | Ins_result x t u } :=
         fix f t :=
           match t with
           | Leaf =>
-            let u := Node Red Leaf x Leaf in
-            exist
-              _ u
-              (fun lo hi h c b rb =>
-                 conj
-                   (Equal.rewrite_bwd
-                      (fun h => _ )
-                      (And.proj1 (rb_inv_leaf rb):h = 0)
-                      (singleton_nearly Red x))
-                   (ins_leaf Red x:Insert x Leaf u))
+            fun rb s =>
+              let u := Node Red Leaf x Leaf in
+              exist
+                _ u
+                (conj
+                   (ins_leaf Red x)
+                   (or_intror
+                      (generalize_height
+                         (fun h => Red_black h Red u)
+                         rb_leaf
+                         (rb_red x rb_leaf rb_leaf)
+                       : forall h, Red_black h Black Leaf -> Red_black h Red u
+                       ))
+                 :Ins_result x Leaf u)
           | Node c t1 y t2 =>
             match S.compare3 x y with
-            | less_than xy => bal_left c t1 (f t1) y t2
-            | equivalent xy yx => sub c t1 y t2 xy yx
-            | greater_than yx => bal_right c t1 y t2 (f t2)
+            | less_than xy =>
+              fun rb s =>
+                match f t1 (left_son_red_black rb) (left_son_sorted s) with
+                | exist _ u1 inv1 =>
+                  match c with
+                  | Red =>
+                    let u := Node Red u1 y t2 in
+                    exist
+                      _ u
+                      (_: Ins_result x _ u)
+                  | Black => _
+                  end
+                end
+            | equivalent xy yx =>_
+            | greater_than yx =>_
             end
           end
     in
-    let mblack: Res0 t -> Insert_result x t := _ in
-    mblack (ins t).
-
-
-
-
-
-
-
-  Definition Insert_result (x:S.t) (t:tree): Type :=
-    {u:tree | Red_black u /\ Insert x t u}.
-
-  Definition insert
-             (x:S.t) (t:tree) (rb:Red_black t) (s:Sorted t)
-    : Insert_result x t :=
-    let Res00 t :=
-        {u |
-         forall lo hi h c,
-           Bounded0 lo t hi ->
-           RB_inv h c t ->
-           RB_nearly_inv h u /\ Insert x t u} in
-    let Res0 t :=
-        {u | RB_nearly u /\ Insert x t u} in
-    let Res t  := Insert_result x t in
-    let ins: forall t, Red_black t -> Sorted t ->  Res0 t :=
-        fix f t :=
-          match t with
-          | Leaf =>
-            fun _ _ =>
-              exist
-                _ (Node Red Leaf x Leaf)
-                (conj
-                   (ex_intro _ 0 (singleton_nearly Red x))
-                   (ins_leaf Red x)
-                )
-          | Node c t1 y t2 =>
-            fun rb sort =>
-              match S.compare3 x y with
-              | less_than xy =>
-                let s1 := And.proj1 (sons_sorted sort) in
-                let s2 := And.proj2 (sons_sorted sort) in
-                _
-                (*Sigma.use
-                  (f t1 _)
-                  (fun t1a
-                       (rbn1:RB_nearly t1a)
-                       (i:Insert x t1 t1a) sb =>
-                     _)*)
-              | equivalent xy zx =>
-                _
-              | greater_than yx =>
-                _
-              end
-          end
-    in
-    let mblack t: Res0 t -> Insert_result x t := _ in
-    _.
-
-
-  Definition insert (x:S.t) (t:RBT): RBT :=
-    let bd t := black_depth (Sigma.value t) in
-    let ins: forall t:RBT, RBN (bd t) := _
-    in
-    let make_black (u:RBN (bd t)): RBT := _ in
-    make_black (ins t).
+    let mblack: forall u, Ins_result x t u -> Insert_result x t := _ in
+    fun rb s => Sigma.use (ins t rb s) (fun u p => mblack u p).
 End M1.
 
 
